update rules

EncRelSeq/Basics/safeexec_lib.v
@@ -33,8 +33,22 @@ Section  safe_rules.
   Context {Σ : Type}.
 
   Ltac destructs  H:= one_destruct Σ (@denosem Σ) H. 
-  
-  Lemma Exec_imply_cont : forall (P P': @asrt Σ)  s ks,
+
+  Lemma highstepend_derive : forall s (P P' : Σ -> Prop),
+  ⊢∃ {{P}} s {{P'}} -> (forall X, Exec P s X -> Exec P' skip X).
+  Proof.
+    intros.
+    unfold valid_angelic_triple, Exec, safe in *.
+    destructs H0. 
+    simpl in *.
+    specialize (H _ H0) as [σₕ' [? ?]].
+    exists σₕ'.
+    splits;auto. 
+    unfold safe,weakestpre, skip;simpl; sets_unfold; simpl;intros.
+    subst.
+    eapply H1;eauto.
+  Qed.
+  Lemma Exec_Seq : forall (P P': @asrt Σ)  s ks,
     (forall X, Exec P s X -> Exec P' skip X) ->
     (forall X, Exec P (seq s ks) X -> Exec P' ks X).
   Proof. 
@@ -59,28 +73,219 @@ Section  safe_rules.
     split;eauto.
   Qed.
 
-  Lemma highstepend_derive : forall s (P P' : Σ -> Prop),
-  ⊢∃ {{P}} s {{P'}} -> (forall X, Exec P s X -> Exec P' skip X).
-  Proof.
-    intros.
-    unfold valid_angelic_triple, Exec, safe in *.
+  Lemma Exec_Pure : forall (P: @asrt Σ) s s' ks,
+    (forall X, Exec P s X -> Exec P s' X) ->
+    (forall X, Exec P (seq s ks) X -> Exec P (seq s' ks) X).
+  Proof. 
+    unfold Exec; sets_unfold;intros.
+    simpl_hdefs.
     destructs H0. 
-    simpl in *.
-    specialize (H _ H0) as [σₕ' [? ?]].
-    exists σₕ'.
-    splits;auto. 
-    unfold safe,weakestpre, skip;simpl; sets_unfold; simpl;intros.
-    subst.
-    eapply H1;eauto.
+    specialize (H (fun x => s.(nrm) st x)).
+    assert ((exists σₕ0 : Σ, P σₕ0 /\ safe σₕ0 s (fun x : Σ => nrm s st x))).
+    { eexists;splits;eauto. 
+      unfold safe. simpl. sets_unfold. unfold weakestpre. auto. }
+    specialize (H H2);clear H2.
+    destructs H.
+    exists st0. split;auto. 
+    unfold weakestpre. sets_unfold.
+    intros. unfold seq in H3. sets_unfold in H3. simpl in H3.
+    destructs H3.
+    apply H1.
+    unfold seq;sets_unfold;simpl.
+    eexists.
+    split;eauto.
+    apply H2. auto.
   Qed.
 
   Lemma highstepseq_derive : forall s (P P' : Σ -> Prop),
-  ⊢∃ {{P}} s {{P'}} -> (forall ks X, Exec P (seq s ks) X -> Exec P' ks X).
+    ⊢∃ {{P}} s {{P'}} -> (forall ks X, Exec P (seq s ks) X -> Exec P' ks X).
   Proof.
     intros * H ks.
-    eapply Exec_imply_cont;eauto.
+    eapply Exec_Seq;eauto.
     eapply highstepend_derive;eauto.
   Qed.
 
-End  safe_rules. 
+
+  Lemma Exec_Assume: forall (P b: @asrt Σ) X,
+    P |-- b ->
+    Exec P (assume b) X -> Exec P skip X.
+  Proof.
+    unfold Exec, derivable1; sets_unfold;intros.
+    simpl_hdefs.
+    destructs H0.
+    eexists.
+    split;eauto.
+    unfold weakestpre in *.  simpl in *.
+    sets_unfold.
+    intros. subst.
+    apply H in H0.
+    apply H1.
+    split;auto.
+  Qed.
+
+  Lemma Exec_Choice_left: forall (P: @asrt Σ) c1 c2 X,
+    Exec P (choice c1 c2) X -> Exec P c1 X.
+  Proof.
+    unfold Exec; sets_unfold; intros.
+    simpl_hdefs.
+    destructs H.
+    eexists.
+    split;eauto.
+    unfold weakestpre in *.  simpl in *.
+    sets_unfold in H0.
+    intros.
+    apply H0. auto.
+  Qed.
+  Lemma Exec_Choice_right: forall (P: @asrt Σ) c1 c2 X,
+    Exec P (choice c1 c2) X -> Exec P c2 X.
+  Proof.
+    unfold Exec; sets_unfold; intros.
+    simpl_hdefs.
+    destructs H.
+    eexists.
+    split;eauto.
+    unfold weakestpre in *.  simpl in *.
+    sets_unfold in H0.
+    intros.
+    apply H0. auto.
+  Qed.
+
+  Lemma Exec_While_End: forall (P b: @asrt Σ) c X,
+    P |-- notB b ->
+    Exec P (while b c) X -> Exec P skip X.
+  Proof.
+    unfold Exec, derivable1; sets_unfold;intros.
+    simpl_hdefs.
+    destructs H0.
+    eexists.
+    split;eauto.
+    unfold weakestpre in *.  simpl in *.
+    sets_unfold.
+    intros. subst.
+    apply H in H0.
+    apply H1.
+    unfold SetsFixedpoints.Lfix. sets_unfold.
+    exists 1.
+    simpl.
+    right.
+    split;auto.
+  Qed.
+
+  Lemma Exec_While_Unroll: forall (P b: @asrt Σ) c X,
+    P |-- b ->
+    Exec P (while b c) X -> Exec P (seq (c) (while b c)) X.
+  Proof.
+    unfold Exec, derivable1; sets_unfold;intros.
+    simpl_hdefs.
+    destructs H0.
+    eexists.
+    split;eauto.
+    unfold weakestpre in *.  simpl in *.
+    sets_unfold.
+    intros. subst.
+    apply H in H0.
+    apply H1.
+    unfold SetsFixedpoints.Lfix in *. sets_unfold.
+    destruct H2 as [st0 [? ?]]. sets_unfold in H3.
+    destruct H3 as [n ?].
+    exists (S n).
+    simpl.
+    left.
+    exists st.
+    split;auto.
+    exists st0.
+    split;auto.
+  Qed.
+
+End  safe_rules.
+
 End  NormalDenoExecLib.
+
+
+From Coq Require Import String.
+From Coq Require Import Arith.Arith.
+From Coq Require Import Arith.PeanoNat.
+From Coq Require Import Logic.FunctionalExtensionality.
+From Coq Require Import Bool.Bool.
+From Coq Require Import Relations.
+
+Import StringSyntax.  (* Optional: allows writing string literals more easily *)
+Local Open Scope string_scope.
+Local Open Scope nat_scope.
+
+
+Module AssignmentRules.
+
+Import normaldeno.
+Import NormalDenoConstructs.
+Import HoareNormalDeno.
+
+Definition Var := string. (* or any identifier type *)
+Definition Val := nat.    (* adjust as needed *)
+
+Definition State := Var -> Val.
+
+(* Expressions are interpreted as state -> value *)
+Definition Expr := State -> Val.
+
+Definition update (σ : State) (x : Var) (v : Val) : State :=
+  fun y => if String.eqb y x then v else σ y.
+
+Definition assign (x : Var) (e : Expr) : @normaldeno.denosem State :=
+  {|
+    normaldeno.nrm := fun σ σ' => σ' = update σ x (e σ);
+  |}.
+
+Definition in_range (v lo hi : Val) := lo <= v <= hi.
+
+Definition nd_assign (x : Var) (e1 e2 : Expr) : @normaldeno.denosem State :=
+  {|
+    normaldeno.nrm := fun σ σ' =>
+      let lo := e1 σ in
+      let hi := e2 σ in
+      in_range (σ' x) lo hi /\
+      (forall y, y <> x -> σ' y = σ y);
+  |}.
+
+Lemma exec_assign:
+  forall (P X : State -> Prop) (x : Var) (e : Expr),
+    Exec (fun σ => P (update σ x (e σ))) (assign x e) X ->
+    Exec P skip X.
+Proof.
+  intros P X x e [σ [HP Hwp]].
+  exists (update σ x (e σ)). split.
+  - apply HP.
+  - intros σ' Hskip. subst. apply Hwp.
+    simpl. simpl in Hskip. sets_unfold in Hskip. auto.
+Qed.
+
+Lemma exec_nd_assign_backward :
+  forall (P X : State -> Prop) (x : Var) (e1 e2 : Expr) (v : Val),
+    (forall σ, P (update σ x v) -> e1 σ <= v <= e2 σ) ->
+    Exec (fun σ => P (update σ x v)) (nd_assign x e1 e2) X ->
+    Exec P skip X.
+Proof.
+  intros P X x e1 e2 v Hv [σ [HP Hwp]].
+  exists (update σ x v). split.
+  - apply HP.
+  - intros σ' Hskip. subst. apply Hwp.
+    simpl.
+    unfold nd_assign. simpl.
+    split.
+    + unfold in_range. sets_unfold in HP. 
+      simpl in Hskip.  sets_unfold in Hskip.  subst.
+      unfold update. 
+      rewrite String.eqb_refl.
+      apply Hv. apply HP.
+    + intros y Hneq.
+      simpl in Hskip.  sets_unfold in Hskip. subst.
+      unfold update. destruct (String.eqb y x) eqn:Heq.
+      * apply String.eqb_eq in Heq. contradiction.
+      * reflexivity.
+Qed.
+
+
+End AssignmentRules.
+
+
+
